WIP

src/ModAdequacy.v
@@ -29,9 +29,9 @@ Section AUX.
   Variable _ident_src: ID.
   Variable _ident_tgt: ID.
 
-  Definition wf_ths {R}
-             (ths_src: @threads _ident_src E1 R)
-             (ths_tgt: @threads _ident_tgt E2 R) :=
+  Definition wf_ths {R0 R1}
+             (ths_src: @threads _ident_src E1 R0)
+             (ths_tgt: @threads _ident_tgt E2 R1) :=
     (alist_proj1 ths_src) = (alist_proj1 ths_tgt).
 
   Lemma ths_find_none_tid_add
@@ -75,11 +75,11 @@ Section ADEQ.
 
   (*invariant for tid_list & threads: tid_list_add threads.proj1 tid tid_list*)
   Theorem local_adequacy
-          R
-          (LSIM: forall (src0: itree srcE R) (tgt0: itree tgtE R),
-              local_sim world_le I src0 tgt0)
-          (ths_src: @threads _ident_src (sE state_src) R)
-          (ths_tgt: @threads _ident_tgt (sE state_tgt) R)
+          R0 R1 (RR: R0 -> R1 -> Prop)
+          (LSIM: forall (src0: itree srcE R0) (tgt0: itree tgtE R1),
+              local_sim world_le I RR src0 tgt0)
+          (ths_src: @threads _ident_src (sE state_src) R0)
+          (ths_tgt: @threads _ident_tgt (sE state_tgt) R1)
           tid src tgt (st_src: state_src) (st_tgt: state_tgt)
           (WFTHS: wf_ths ths_src ths_tgt)
           (THSRC: threads_find tid ths_src = None)
@@ -87,13 +87,69 @@ Section ADEQ.
           (INV: forall im_tgt, exists im_src o w,
               I (alist_proj1 ths_src, im_src, im_tgt, st_src, st_tgt, o, w))
     :
-    gsim wf_src wf_tgt (@eq R) false false
+    gsim wf_src wf_tgt RR false false
          (interp_all st_src ths_src tid src)
          (interp_all st_tgt ths_tgt tid tgt).
   Proof.
     ii. specialize (INV mt). des. rename im_src into ms. exists ms.
     pose proof (ths_find_none_tid_add ths_src tid THSRC) as TADD. 
     unfold local_sim in LSIM. specialize (LSIM src tgt _ _ _ _ _ _ _ INV tid _ TADD).
+    ginit. revert_until I. gcofix CIH. i.
+    remember (tid :: alist_proj1 ths_src) as tlist.
+    match goal with
+    | LSIM: lsim _ _ tid ?_LRR _ _ _ _ ?_shr |- _ => remember _LRR as LRR; remember _shr as shr
+    end.
+    remember false as ps in LSIM at 1. remember false as pt in LSIM at 1.
+    (* remember tid as tid0 in LSIM. *)
+    punfold LSIM.
+    2:{ ii. eapply pind8_mon_gen; eauto. i. eapply __lsim_mon; eauto. }
+    move LSIM before CIH. revert_until LSIM.
+    eapply pind8_acc in LSIM.
+    { instantiate (1:= (fun R0 R1 (LRR: R0 -> R1 -> tid_list * imap wf_src * imap wf_tgt * state_src * state_tgt * T wf_src * world -> Prop) ps pt (src: itree srcE R0) (tgt: itree tgtE R1) shr =>
+                          forall (RR : R0 -> R1 -> Prop) (ths_src : threads (sE state_src)) (st_src : state_src) (st_tgt : state_tgt) 
+                            (mt : imap wf_tgt) (ms : imap wf_src) (o : T wf_src) (w : world) (tlist : list nat),
+                            tlist = tid :: alist_proj1 ths_src ->
+                            LRR = local_RR world_le I RR tid ->
+                            shr = (tlist, ms, mt, st_src, st_tgt, o, w) ->
+                            ps = false ->
+                            pt = false ->
+                            forall ths_tgt : threads (sE state_tgt),
+                              wf_ths ths_src ths_tgt ->
+                              threads_find tid ths_src = None ->
+                              threads_find tid ths_tgt = None ->
+                              I (alist_proj1 ths_src, ms, mt, st_src, st_tgt, o, w) ->
+                              tid_list_add (alist_proj1 ths_src) tid tlist ->
+                              gpaco9 (_sim (wft:=wf_tgt)) (cpn9 (_sim (wft:=wf_tgt))) bot9 r R0 R1 RR false ms false mt (interp_all st_src ths_src tid src)
+                                     (interp_all st_tgt ths_tgt tid tgt))) in LSIM. auto. }
+    (* { instantiate (1:= *)
+    (*                  (fun R0 R1 (LRR: R0 -> R1 -> tid_list * imap wf_src * imap wf_tgt * state_src * state_tgt * T wf_src * world -> Prop) ps pt (src: itree srcE R0) (tgt: itree tgtE R1) shr => *)
+    (*                     forall (RR : R0 -> R1 -> Prop) (ths_src : threads (sE state_src)) (tid : nat) (st_src : state_src) (st_tgt : state_tgt) *)
+    (*                       (mt : imap wf_tgt) (ms : imap wf_src) (o : T wf_src) (w : world) (tlist : list nat), *)
+    (*                       tlist = tid :: alist_proj1 ths_src -> *)
+    (*                       LRR = local_RR world_le I RR tid -> *)
+    (*                       shr = (tlist, ms, mt, st_src, st_tgt, o, w) -> *)
+    (*                       ps = false -> *)
+    (*                       pt = false -> *)
+    (*                       tid0 = tid -> *)
+    (*                       forall ths_tgt : threads (sE state_tgt), *)
+    (*                         wf_ths ths_src ths_tgt -> *)
+    (*                         threads_find tid ths_src = None -> *)
+    (*                         threads_find tid ths_tgt = None -> *)
+    (*                         I (alist_proj1 ths_src, ms, mt, st_src, st_tgt, o, w) -> *)
+    (*                         tid_list_add (alist_proj1 ths_src) tid tlist -> *)
+    (*                         gpaco9 (_sim (wft:=wf_tgt)) (cpn9 (_sim (wft:=wf_tgt))) bot9 r R0 R1 RR false ms false mt (interp_all st_src ths_src tid src) *)
+    (*                                (interp_all st_tgt ths_tgt tid tgt))) in LSIM. auto. } *)
+
+    clear R0 R1 LRR ps pt src tgt shr LSIM. i.
+    rename x0 into R0, x1 into R1, x2 into LRR, x3 into ps, x4 into pt, x5 into src, x6 into tgt, x7 into shr, PR into LSIM.
+    ss. i. clear DEC.
+
+
+
+
+
+
+                        
 
 
   Abort.
