src/ModSimPico.v
@@ -232,22 +232,22 @@ Section PRIMIVIESIM.
     ii. eapply __lsim_mon; eauto.
   Qed.
 
-  Definition local_RR {R} tid :=
-    fun (r_src r_tgt: R) '(ths2, im_src1, im_tgt1, st_src1, st_tgt1, o1, w1) =>
+  Definition local_RR {R0 R1} (RR: R0 -> R1 -> Prop) tid :=
+    fun (r_src: R0) (r_tgt: R1) '(ths2, im_src1, im_tgt1, st_src1, st_tgt1, o1, w1) =>
       exists ths3 w2,
         (<<THS: tid_list_remove ths2 tid ths3>>) /\
           (<<WORLD: world_le w1 w2>>) /\
           (<<INV: I (ths3, im_src1, im_tgt1, st_src1, st_tgt1, o1, w2)>>) /\
-          (<<RET: r_src = r_tgt>>).
+          (<<RET: RR r_src r_tgt>>).
 
-  Definition local_sim {R} src tgt :=
+  Definition local_sim {R0 R1} (RR: R0 -> R1 -> Prop) src tgt :=
     forall ths0 im_src0 im_tgt0 st_src0 st_tgt0 o0 w0
       (INV: I (ths0, im_src0, im_tgt0, st_src0, st_tgt0, o0, w0))
       tid ths1
       (THS: tid_list_add ths0 tid ths1),
       lsim
         tid
-        (@local_RR R tid)
+        (@local_RR R0 R1 RR tid)
         false false
         src tgt
         (ths1, im_src0, im_tgt0, st_src0, st_tgt0, o0, w0).
@@ -277,7 +277,7 @@ Module ModSim.
           init: forall im_tgt, exists im_src o w,
             I ([], im_src, im_tgt, md_src.(Mod.st_init), md_tgt.(Mod.st_init), o, w);
 
-          funs: forall fn args, local_sim world_le I (md_src.(Mod.funs) fn args) (md_tgt.(Mod.funs) fn args);
+          funs: forall fn args, local_sim world_le I (@eq Val) (md_src.(Mod.funs) fn args) (md_tgt.(Mod.funs) fn args);
         }.
 
     (* Record local_sim: Prop := *)
